theories/Syntax/UnOps.v
@@ -1,0 +1,202 @@
+(******************************************************************************)
+(* Copyright (c) 2023 Steven Keuchel                                          *)
+(* All rights reserved.                                                       *)
+(*                                                                            *)
+(* Redistribution and use in source and binary forms, with or without         *)
+(* modification, are permitted provided that the following conditions are     *)
+(* met:                                                                       *)
+(*                                                                            *)
+(* 1. Redistributions of source code must retain the above copyright notice,  *)
+(*    this list of conditions and the following disclaimer.                   *)
+(*                                                                            *)
+(* 2. Redistributions in binary form must reproduce the above copyright       *)
+(*    notice, this list of conditions and the following disclaimer in the     *)
+(*    documentation and/or other materials provided with the distribution.    *)
+(*                                                                            *)
+(* THIS SOFTWARE IS PROVIDED BY THE COPYRIGHT HOLDERS AND CONTRIBUTORS        *)
+(* "AS IS" AND ANY EXPRESS OR IMPLIED WARRANTIES, INCLUDING, BUT NOT LIMITED  *)
+(* TO, THE IMPLIED WARRANTIES OF MERCHANTABILITY AND FITNESS FOR A PARTICULAR *)
+(* PURPOSE ARE DISCLAIMED. IN NO EVENT SHALL THE COPYRIGHT HOLDER OR          *)
+(* CONTRIBUTORS BE LIABLE FOR ANY DIRECT, INDIRECT, INCIDENTAL, SPECIAL,      *)
+(* EXEMPLARY, OR CONSEQUENTIAL DAMAGES (INCLUDING, BUT NOT LIMITED TO,        *)
+(* PROCUREMENT OF SUBSTITUTE GOODS OR SERVICES; LOSS OF USE, DATA, OR         *)
+(* PROFITS; OR BUSINESS INTERRUPTION) HOWEVER CAUSED AND ON ANY THEORY OF     *)
+(* LIABILITY, WHETHER IN CONTRACT, STRICT LIABILITY, OR TORT (INCLUDING       *)
+(* NEGLIGENCE OR OTHERWISE) ARISING IN ANY WAY OUT OF THE USE OF THIS         *)
+(* SOFTWARE, EVEN IF ADVISED OF THE POSSIBILITY OF SUCH DAMAGE.               *)
+(******************************************************************************)
+
+From Coq Require Import
+  Arith.PeanoNat
+  ZArith.BinInt.
+From Equations Require Import
+  Equations.
+From Katamaran Require Import
+  Bitvector
+  Context
+  Prelude
+  Syntax.TypeDecl.
+
+Import ctx.notations.
+
+Local Set Implicit Arguments.
+Local Set Transparent Obligations.
+
+Module uop.
+
+  Import ty.
+
+  Section WithTypeDecl.
+    Context {TDC : TypeDeclKit}.
+
+    Variant UnOp : Ty -> Ty -> Set :=
+    | inl {σ1 σ2 : Ty}  : UnOp σ1 (sum σ1 σ2)
+    | inr {σ1 σ2 : Ty}  : UnOp σ2 (sum σ1 σ2)
+    | neg               : UnOp int int
+    | not               : UnOp bool bool
+    | sext {m n} {p : IsTrue (m <=? n)} : UnOp (bvec m) (bvec n)
+    | zext {m n} {p : IsTrue (m <=? n)} : UnOp (bvec m) (bvec n)
+    | get_slice_int {n} : UnOp int (bvec n)
+    | unsigned {n}      : UnOp (bvec n) int
+    | truncate {n} (m : nat) {p : IsTrue (m <=? n)} : UnOp (bvec n) (bvec m)
+    | vector_subrange {n} (s l : nat) {p : IsTrue (s + l <=? n)} : UnOp (bvec n) (bvec l)
+    | negate {n}        : UnOp (bvec n) (bvec n).
+    Set Transparent Obligations.
+    Derive Signature for UnOp.
+    Derive NoConfusion for UnOp.
+
+    Import Sigma_Notations.
+
+    Definition UnOpTel : Set :=
+      Σ i : (Σ σ1 : Ty, Ty), UnOp i.1 i.2.
+
+    Definition unoptel_inl (σ1 σ2 : Ty) : UnOpTel :=
+      ((σ1, sum σ1 σ2), inl).
+    Definition unoptel_inr (σ1 σ2 : Ty) : UnOpTel :=
+      ((σ2, sum σ1 σ2), inr).
+    Definition unoptel_sext {m n} {p : IsTrue (m <=? n)} : UnOpTel :=
+      ((bvec m, bvec n), sext).
+    Definition unoptel_zext {m n} {p : IsTrue (m <=? n)} : UnOpTel :=
+      ((bvec m, bvec n), sext).
+    Definition unoptel_get_slice_int (n : nat) : UnOpTel :=
+      ((int,bvec n), get_slice_int).
+    Definition unoptel_unsigned (n : nat) : UnOpTel :=
+      ((bvec n,int), unsigned).
+    Definition unoptel_negate (n : nat) : UnOpTel :=
+      ((bvec n,bvec n), negate).
+
+  End WithTypeDecl.
+
+  Section WithTypeDef.
+    Context {TDC : TypeDeclKit}.
+    Context {TDN : TypeDenoteKit TDC}.
+    Context {TDF : TypeDefKit TDN}.
+    Import Sigma_Notations.
+
+    Definition unoptel_eq_dec_sext {m1 n1 m2 n2}
+      {p1 : IsTrue (m1 <=? n1)} {p2 : IsTrue (m2 <=? n2)} :
+      dec_eq (A := UnOpTel) ((bvec m1, bvec n1), sext) ((bvec m2, bvec n2), sext).
+    Proof.
+      destruct (eq_dec m1 m2). destruct (eq_dec n1 n2).
+      { subst. left. f_equal. f_equal. apply IsTrue.proof_irrelevance. }
+      all: right; intros Heq; now dependent elimination Heq.
+    Defined.
+
+    Definition unoptel_eq_dec_zext {m1 n1 m2 n2}
+      {p1 : IsTrue (m1 <=? n1)} {p2 : IsTrue (m2 <=? n2)} :
+      dec_eq (A := UnOpTel) ((bvec m1, bvec n1), zext) ((bvec m2, bvec n2), zext).
+    Proof.
+      destruct (eq_dec m1 m2). destruct (eq_dec n1 n2).
+      { subst. left. f_equal. f_equal. apply IsTrue.proof_irrelevance. }
+      all: right; intros Heq; now dependent elimination Heq.
+    Defined.
+
+    Definition unoptel_eq_dec_truncate {m1 n1 m2 n2}
+      {p1 : IsTrue (m1 <=? n1)} {p2 : IsTrue (m2 <=? n2)} :
+      dec_eq (A := UnOpTel)
+        ((bvec n1, bvec m1), truncate m1)
+        ((bvec n2, bvec m2), truncate m2).
+    Proof.
+      destruct (eq_dec n1 n2). destruct (eq_dec m1 m2).
+      { subst. left. f_equal. f_equal. apply IsTrue.proof_irrelevance. }
+      all: right; intros Heq; now dependent elimination Heq.
+    Defined.
+
+    Definition unoptel_eq_dec_subrange {n1 s1 l1 n2 s2 l2}
+      {p1 : IsTrue (s1 + l1 <=? n1)} {p2 : IsTrue (s2 + l2 <=? n2)} :
+      dec_eq (A := UnOpTel)
+        ((bvec n1, bvec l1), vector_subrange s1 l1)
+        ((bvec n2, bvec l2), vector_subrange s2 l2).
+    Proof.
+      destruct (eq_dec n1 n2). destruct (eq_dec l1 l2). destruct (eq_dec s1 s2).
+      { subst. left. f_equal. f_equal. apply IsTrue.proof_irrelevance. }
+      all: right; intros Heq; now dependent elimination Heq.
+    Defined.
+
+    Definition unoptel_eq_dec {σ1 σ2 τ1 τ2 : Ty}
+      (op1 : UnOp σ1 σ2) (op2 : UnOp τ1 τ2) :
+      dec_eq (A := UnOpTel) ((σ1,σ2),op1) ((τ1,τ2),op2) :=
+      let ninv := @noConfusion_inv UnOpTel (NoConfusionPackage_UnOp) in
+      match op1 , op2 with
+      | @inl _ σ1 σ2 , @inl _ τ1 τ2  =>
+          f_equal2_dec unoptel_inl (ninv _ _) (eq_dec σ1 τ1) (eq_dec σ2 τ2)
+      | @inr _ σ1 σ2 , @inr _ τ1 τ2  =>
+          f_equal2_dec unoptel_inr (ninv _ _) (eq_dec σ1 τ1) (eq_dec σ2 τ2)
+      | neg  , neg  => left eq_refl
+      | not  , not  => left eq_refl
+      | sext , sext => unoptel_eq_dec_sext
+      | zext , zext => unoptel_eq_dec_zext
+      | @get_slice_int _ m , @get_slice_int _ n =>
+          f_equal_dec unoptel_get_slice_int (ninv _ _) (eq_dec m n)
+      | @unsigned _ m , @unsigned _ n =>
+          f_equal_dec unoptel_unsigned (ninv _ _) (eq_dec m n)
+      | truncate m1 , truncate m2 => unoptel_eq_dec_truncate
+      | vector_subrange s1 l1 , vector_subrange s2 l2 => unoptel_eq_dec_subrange
+      | @negate _ m , @negate _ n =>
+          f_equal_dec unoptel_negate (ninv _ _) (eq_dec m n)
+      | _ , _ => right (ninv _ _)
+      end.
+
+    Inductive OpEq {σ1 σ2} (op1 : UnOp σ1 σ2) : forall {τ1 τ2}, UnOp τ1 τ2 -> Prop :=
+    | opeq_refl : OpEq op1 op1.
+    Derive Signature for OpEq.
+    Global Arguments opeq_refl {_ _ _}.
+
+    Lemma eqdep_dec {σ1 σ2 τ1 τ2} (op1 : UnOp σ1 σ2) (op2 : UnOp τ1 τ2) :
+      {OpEq op1 op2} + {~ OpEq op1 op2}.
+    Proof.
+      destruct (unoptel_eq_dec op1 op2).
+      - left. dependent elimination e. constructor.
+      - right. intro e. apply n. dependent elimination e. reflexivity.
+    Defined.
+
+    Local Set Equations With UIP.
+    Instance eq_dec_unop {σ1 σ2} : EqDec (UnOp σ1 σ2).
+    Proof.
+      intros x y.
+      destruct (unoptel_eq_dec x y) as [p|p].
+      - left. dependent elimination p. reflexivity.
+      - right. congruence.
+    Defined.
+
+    Definition eval {σ1 σ2 : Ty} (op : UnOp σ1 σ2) : Val σ1 -> Val σ2 :=
+      match op in UnOp σ1 σ2 return Val σ1 -> Val σ2 with
+      | inl                 => Datatypes.inl
+      | inr                 => Datatypes.inr
+      | neg                 => Z.opp
+      | not                 => negb
+      | sext                => fun v => bv.sext v
+      | zext                => fun v => bv.zext v
+      | get_slice_int       => bv.of_Z
+      | unsigned            => fun v => bv.unsigned v
+      | truncate m          => fun v => bv.truncate m v
+      | vector_subrange s l => bv.vector_subrange s l
+      | negate              => bv.negate
+      end.
+
+  End WithTypeDef.
+  #[export] Existing Instance eq_dec_unop.
+
+End uop.
+#[export] Existing Instance uop.eq_dec_unop.
+Export uop (UnOp).
